theories/typing/lib/smallvec/smallvec_basic.v
@@ -9,7 +9,7 @@ Implicit Type 𝔄 𝔅: syn_type.
 Section smallvec_basic.
   Context `{!typeG Σ}.
 
-  Global Instance smallvec_type_ne 𝔄 n : TypeNonExpansive (smallvec_ty (𝔄:=𝔄) n).
+  Global Instance smallvec_type_ne 𝔄 n : TypeNonExpansive (smallvec (𝔄:=𝔄) n).
   Proof.
     split.
     - by apply type_lft_morphism_id_like.
@@ -18,14 +18,14 @@ Section smallvec_basic.
     - move=>/= > ->*. by do 18 f_equiv; [|f_equiv].
   Qed.
 
-  Global Instance smallvec_send {𝔄} n (ty: type 𝔄) : Send ty → Send (smallvec_ty n ty).
+  Global Instance smallvec_send {𝔄} n (ty: type 𝔄) : Send ty → Send (smallvec n ty).
   Proof. move=> ?>/=. by do 24 f_equiv. Qed.
 
-  Global Instance smallvec_sync {𝔄} n (ty: type 𝔄) : Sync ty → Sync (smallvec_ty n ty).
+  Global Instance smallvec_sync {𝔄} n (ty: type 𝔄) : Sync ty → Sync (smallvec n ty).
   Proof. move=> ?>/=. by do 18 f_equiv; [|f_equiv]. Qed.
 
   Lemma smallvec_resolve {𝔄} n (ty: type 𝔄) Φ E L :
-    resolve E L ty Φ → resolve E L (smallvec_ty n ty) (lforall Φ).
+    resolve E L ty Φ → resolve E L (smallvec n ty) (lforall Φ).
   Proof.
     iIntros (????[|]???) "LFT PROPH E L svec/="; [done|].
     iDestruct "svec" as (b ?????(->&?&->)) "big". case b=>/=.
@@ -38,11 +38,11 @@ Section smallvec_basic.
   Qed.
 
   Lemma smallvec_resolve_just {𝔄} n (ty: type 𝔄) E L :
-    resolve E L ty (const True) → resolve E L (smallvec_ty n ty) (const True).
+    resolve E L ty (const True) → resolve E L (smallvec n ty) (const True).
   Proof. move=> ?. apply resolve_just. Qed.
 
   Lemma smallvec_real {𝔄 𝔅} n (ty: type 𝔄) (f: 𝔄 → 𝔅) E L :
-    real E L ty f → real (𝔅:=listₛ _) E L (smallvec_ty n ty) (map f).
+    real E L ty f → real (𝔅:=listₛ _) E L (smallvec n ty) (map f).
   Proof.
     move=> Rl. split; iIntros (???[|]) "*% LFT E L svec//=".
     - iDestruct "svec" as (b ?????(->&?&->)) "big". case b=>/=.
@@ -76,7 +76,7 @@ Section smallvec_basic.
   Qed.
 
   Lemma smallvec_subtype {𝔄 𝔅} (f: 𝔄 → 𝔅) n ty ty' E L :
-    subtype E L ty ty' f → subtype E L (smallvec_ty n ty) (smallvec_ty n ty') (map f).
+    subtype E L ty ty' f → subtype E L (smallvec n ty) (smallvec n ty') (map f).
   Proof.
     iIntros (Sub ?) "L". iDestruct (Sub with "L") as "#Sub". iIntros "!> E".
     iDestruct ("Sub" with "E") as "(%EqSz &?&#?&#?)".
@@ -95,7 +95,7 @@ Section smallvec_basic.
   Qed.
   Lemma smallvec_eqtype {𝔄 𝔅} (f: 𝔄 → 𝔅) g n ty ty' E L :
     eqtype E L ty ty' f g →
-    eqtype E L (smallvec_ty n ty) (smallvec_ty n ty') (map f) (map g).
+    eqtype E L (smallvec n ty) (smallvec n ty') (map f) (map g).
   Proof. move=> [??]. split; by apply smallvec_subtype. Qed.
 
   (* smallvec_new *)
